clightplus/mem/ClightPlusMem1.v
@@ -8,7 +8,6 @@ Require Import PCM IPM.
 Require Import HoareDef STB.
 Require Import ClightPlusSkel.
 Require Import ClightPlusExprgen.
-Require Import ClightPlusgen.
 From compcert Require Import Floats Integers Values Memory AST Ctypes Clight Clightdefs.
 Require Import List.
 
